updated documentation and last example

progs64/verif_incr_gen.v
@@ -45,6 +45,8 @@ Definition t_counter := Tstruct _counter noattr.
 Definition cptr_lock_inv g ctr :=
   EX z : nat, field_at Ews t_counter [StructField _ctr] (Vint (Int.repr (Z.of_nat z))) ctr * ghost_ref z g.
 
+Definition ctr_handle sh h g ctr n := lock_inv sh h (cptr_lock_inv g ctr) * ghost_part sh n g.
+
 Definition init_ctr_spec :=
  DECLARE _init_ctr
   WITH gv: globals
@@ -59,7 +61,7 @@ Definition init_ctr_spec :=
          LOCAL ()
          SEP (library.mem_mgr gv;
               field_at Ews t_counter [StructField _lock] (ptr_of h) (gv _c); spacer Ews 4 8 (gv _c);
-              lock_inv Tsh h (cptr_lock_inv g (gv _c)); ghost_part Tsh O g).
+              ctr_handle Tsh h g (gv _c) O).
 
 Definition dest_ctr_spec :=
  DECLARE _dest_ctr
@@ -69,7 +71,7 @@ Definition dest_ctr_spec :=
          PARAMS ()
          GLOBALS (gv)
          SEP (field_at Ews t_counter [StructField _lock] (ptr_of h) (gv _c); spacer Ews 4 8 (gv _c);
-              lock_inv Tsh h (cptr_lock_inv g (gv _c)); ghost_part Tsh v g)
+              ctr_handle Tsh h g (gv _c) v)
   POST [ tvoid ]
          PROP ()
          LOCAL ()
@@ -77,39 +79,40 @@ Definition dest_ctr_spec :=
 
 Definition incr_spec :=
  DECLARE _incr
-  WITH sh1 : share, sh : share, h : lock_handle, gsh : share, g : gname, n : nat, gv: globals
+  WITH sh1 : share, sh : share, h : lock_handle, g : gname, n : nat, gv: globals
   PRE [ ]
-         PROP  (readable_share sh1; sh <> Share.bot; gsh <> Share.bot)
+         PROP  (readable_share sh1; sh <> Share.bot)
          PARAMS ()
          GLOBALS (gv)
-         SEP (field_at sh1 t_counter [StructField _lock] (ptr_of h) (gv _c); lock_inv sh h (cptr_lock_inv g (gv _c)); ghost_part gsh n g)
+         SEP (field_at sh1 t_counter [StructField _lock] (ptr_of h) (gv _c);
+              ctr_handle sh h g (gv _c) n)
   POST [ tvoid ]
          PROP ()
          LOCAL ()
-         SEP (field_at sh1 t_counter [StructField _lock] (ptr_of h) (gv _c); lock_inv sh h (cptr_lock_inv g (gv _c)); ghost_part gsh (S n) g).
+         SEP (field_at sh1 t_counter [StructField _lock] (ptr_of h) (gv _c);
+              ctr_handle sh h g (gv _c) (S n)).
 
 
-Definition thread_lock_R sh1 sh gsh g ctr lockc :=
-  field_at sh1 t_counter [StructField _lock] (ptr_of lockc) ctr * lock_inv sh lockc (cptr_lock_inv g ctr) * ghost_part gsh 1%nat g.
+Definition thread_lock_R sh1 sh g ctr lockc :=
+  field_at sh1 t_counter [StructField _lock] (ptr_of lockc) ctr * ctr_handle sh lockc g ctr 1%nat.
 
-Definition thread_lock_inv sh1 tsh sh gsh g ctr lockc lockt :=
-  selflock (thread_lock_R sh1 sh gsh g ctr lockc) tsh lockt.
+Definition thread_lock_inv sh1 tsh sh g ctr lockc lockt :=
+  selflock (thread_lock_R sh1 sh g ctr lockc) tsh lockt.
 
 Definition thread_func_spec :=
  DECLARE _thread_func
-  WITH y : val, x : share * share * lock_handle * share * lock_handle * share * gname * val * globals
+  WITH y : val, x : share * share * lock_handle * share * lock_handle * gname * globals
   PRE [ tptr tvoid ]
-         let '(sh1, tsh, ht, sh, h, gsh, g, l, gv) := x in
-         PROP  (readable_share sh1; tsh <> Share.bot; sh <> Share.bot; gsh <> Share.bot)
-         PARAMS (ptr_of ht)
+         let '(sh1, tsh, ht, sh, h, g, gv) := x in
+         PROP  (readable_share sh1; tsh <> Share.bot; sh <> Share.bot; ptr_of ht = y)
+         PARAMS (y)
          GLOBALS (gv)
          SEP   (field_at sh1 t_counter [StructField _lock] (ptr_of h) (gv _c); 
-                lock_inv sh h (cptr_lock_inv g (gv _c));
-                ghost_part gsh O g;
-                lock_inv tsh ht (thread_lock_inv sh1 tsh sh gsh g (gv _c) h ht))
+                ctr_handle sh h g (gv _c) O;
+                lock_inv tsh ht (thread_lock_inv sh1 tsh sh g (gv _c) h ht))
   POST [ tint ]
          PROP ()
-         LOCAL ()
+         RETURN (Vint Int.zero)
          SEP ().
 
 Definition main_spec :=
@@ -133,17 +136,27 @@ Proof.
 Qed.
 #[export] Hint Resolve ctr_inv_exclusive : core.
 
-Lemma thread_inv_exclusive : forall sh1 sh gsh g ctr lock,
-  exclusive_mpred (thread_lock_R sh1 sh gsh g ctr lock).
+Lemma thread_inv_exclusive : forall sh1 sh g ctr lock,
+  exclusive_mpred (thread_lock_R sh1 sh g ctr lock).
 Proof.
   intros; unfold thread_lock_R.
   apply exclusive_sepcon2; unfold exclusive_mpred.
-  unfold ghost_part, ghosts.ghost_part; rewrite own_op'; Intros x.
+  unfold ctr_handle, ghost_part, ghosts.ghost_part.
+  sep_apply own_op'; Intros x.
   destruct H as [H _]; hnf in H.
   destruct x as ([(?, ?)|], ?); try contradiction; simpl in H.
   destruct H as (? & _ & J & _); apply sepalg.join_self, identity_share_bot in J; contradiction.
 Qed.
 #[export] Hint Resolve thread_inv_exclusive : core.
+
+Lemma ctr_handle_share_join : forall sh1 sh2 sh h g ctr v1 v2, sh1 <> Share.bot -> sh2 <> Share.bot -> sepalg.join sh1 sh2 sh ->
+  ctr_handle sh1 h g ctr v1 * ctr_handle sh2 h g ctr v2 = ctr_handle sh h g ctr (v1 + v2)%nat.
+Proof.
+  intros; unfold ctr_handle.
+  erewrite (sepcon_comm (lock_inv _ _ _)), <- sepcon_assoc, (sepcon_assoc (ghost_part _ _ _)), lock_inv_share_join by eauto.
+  unfold ghost_part; erewrite (sepcon_comm (ghosts.ghost_part _ _ _)), sepcon_assoc, ghost_part_join; eauto.
+  reflexivity.
+Qed.
 
 Lemma body_init_ctr: semax_body Vprog Gprog f_init_ctr init_ctr_spec.
 Proof.
@@ -163,12 +176,13 @@ Proof.
     unfold ghost_both; rewrite <- ghost_part_ref_join.
     unfold_data_at (data_at _ _ _ _).
     unfold ghost_ref; Exists O; entailer!. }
-  unfold ghost_part; Exists h g; entailer!.
+  unfold ctr_handle, ghost_part; Exists h g; entailer!.
 Qed.
 
 Lemma body_dest_ctr: semax_body Vprog Gprog f_dest_ctr dest_ctr_spec.
 Proof.
   start_function.
+  unfold ctr_handle; Intros.
   forward.
   forward_call (Tsh, h, cptr_lock_inv g (gv _c)).
   forward.
@@ -186,6 +200,7 @@ Qed.
 Lemma body_incr: semax_body Vprog Gprog f_incr incr_spec.
 Proof.
   start_function.
+  unfold ctr_handle; Intros.
   forward.
   forward_call (sh, h, cptr_lock_inv g (gv _c)).
   unfold cptr_lock_inv at 2; simpl.
@@ -194,7 +209,7 @@ Proof.
   forward.
   forward.
   gather_SEP (ghost_part _ _ _) (ghost_ref _ _).
-  viewshift_SEP 0 (ghost_part gsh (S n) g * ghost_ref (S z) g).
+  viewshift_SEP 0 (ghost_part sh (S n) g * ghost_ref (S z) g).
   { go_lower.
     unfold ghost_part, ghost_ref; rewrite !ghost_part_ref_join.
     eapply derives_trans, bupd_fupd.
@@ -205,7 +220,7 @@ Proof.
     rewrite Nat2Z.inj_succ.
     entailer!. }
   forward.
-  cancel.
+  unfold ctr_handle; cancel.
 Qed.
 
 Lemma body_thread_func : semax_body Vprog Gprog f_thread_func thread_func_spec.
@@ -213,24 +228,13 @@ Proof.
   start_function.
   Intros.
   forward.
-  forward_call (sh1, sh, h, gsh, g, O, gv).
-  forward_call release_self (tsh, ht, thread_lock_R sh1 sh gsh g (gv _c) h).
+  forward_call (sh1, sh, h, g, O, gv).
+  forward_call release_self (tsh, ht, thread_lock_R sh1 sh g (gv _c) h).
   { unfold thread_lock_inv, selflock, thread_lock_R; cancel. }
   forward.
 Qed.
 
 Definition N := 5.
-
-Lemma ghost_part_share_join : forall g sh1 sh2 sh n1 n2, sh1 <> Share.bot -> sh2 <> Share.bot ->
-  sepalg.join sh1 sh2 sh ->
-  ghost_part sh1 n1 g * ghost_part sh2 n2 g = ghost_part sh (n1 + n2)%nat g.
-Proof.
-  intros.
-  symmetry; apply own_op.
-  hnf; simpl.
-  repeat (split; auto).
-  constructor.
-Qed.
 
 Lemma body_main:  semax_body Vprog Gprog f_main main_spec.
 Proof.
@@ -245,120 +249,95 @@ Proof.
   destruct (split_shares (Z.to_nat N) Tsh) as (gsh0 & gshs & ? & ? & ? & Hgshs); auto.
   rewrite Z2Nat.id in * by (unfold N; computable).
   assert_PROP (field_compatible (tarray (tptr t_lock) N) [] v_thread_lock) by entailer!.
-  set (thread_lock i := offset_val (sizeof (tptr t_lock) * i) v_thread_lock).
-  forward_for_simple_bound N (EX i : Z, EX sh : share, EX gsh : share,
+  assert (N <= Int.max_signed) by computable.
+  forward_for_simple_bound N (EX i : Z, EX sh : share, EX gsh : share, EX ll : list lock_handle,
     PROP (sepalg_list.list_join sh0 (sublist i N shs) sh;
-          sepalg_list.list_join gsh0 (sublist i N gshs) gsh) LOCAL (gvars gv)
-    SEP (lock_inv sh (gv _ctr_lock) (cptr_lock_inv g (gv _ctr));
-         ghost_part g gsh O;
-         iter_sepcon (fun j => lock_inv sh2 (thread_lock j)
-           (thread_lock_inv sh1 (Znth j shs) (Znth j gshs) g (gv _ctr) (gv _ctr_lock) (thread_lock j)))
+          sepalg_list.list_join gsh0 (sublist i N gshs) gsh;
+          Zlength ll = i; Forall isptr (map ptr_of ll))
+    LOCAL (lvar _thread_lock (tarray (tptr t_lock) N) v_thread_lock; gvars gv)
+    SEP (library.mem_mgr gv; field_at sh t_counter (DOT _lock) (ptr_of h) (gv _c);
+         spacer Ews 4 8 (gv _c); ctr_handle gsh h g (gv _c) O;
+         iter_sepcon (fun j => lock_inv gsh1 (Znth j ll)
+           (thread_lock_inv (Znth j shs) gsh2 (Znth j gshs) g (gv _c) h (Znth j ll)))
            (upto (Z.to_nat i));
-         data_at_ Ews (tarray tlock (N - i)) (thread_lock i))).
-  { unfold N; computable. }
-  { Exists Ews Tsh.
-    subst thread_lock.
+         data_at Tsh (tarray (tptr t_lock) N) (map ptr_of ll ++ repeat Vundef (Z.to_nat (N - i))) v_thread_lock; has_ext tt))%assert.
+  { Exists Ews Tsh (@nil lock_handle).
     rewrite !sublist_same by auto; entailer!.
-    apply derives_refl. }
+    rewrite data_at__eq; apply derives_refl. }
   { (* first loop *)
+    forward_call (gv, fun ht => thread_lock_inv (Znth i shs) gsh2 (Znth i gshs) g (gv _c) h ht).
+    Intros ht.
     forward.
-    simpl sem_binary_operation'.
-    replace (force_val _) with (thread_lock i)
-      by (rewrite sem_add_pi_ptr_special; auto; unfold N in *; rep_lia).
-    rewrite data_at__tarray.
-    destruct (Z.to_nat (N - i)) eqn: Hi.
-    { rewrite Z2Nat.inj_sub, Nat.sub_0_le in Hi by lia.
-      apply Z2Nat.inj_le in Hi; lia. }
-    simpl.
-    setoid_rewrite split2_data_at_Tarray_app with (v1 := [default_val tlock]);
-      rewrite ?Zlength_cons, ?Zlength_nil, ?Zlength_list_repeat'; auto.
-    erewrite data_at_singleton_array_eq by eauto.
-    forward_call (thread_lock i, Ews, thread_lock_inv sh1 (Znth i shs) (Znth i gshs) g
-      (gv _ctr) (gv _ctr_lock) (thread_lock i)).
-    { cancel. }
-    rewrite sublist_next in H9, H10 by lia.
-    inv H9; inv H10.
-    assert (readable_share (Znth i shs)) by (apply Forall_Znth; auto; lia).
-    assert (Znth i gshs <> Share.bot).
+    assert_PROP (0 <= i < Zlength (map ptr_of ll ++ repeat Vundef (Z.to_nat (N - i)))) as Hi.
+    { entailer!. rewrite Zlength_app, Zlength_map, Zlength_repeat, Zplus_minus by lia; auto. }
+    forward.
+    { rewrite upd_Znth_same by auto; entailer!. }
+    rewrite upd_Znth_same by auto.
+    assert (readable_share (Znth (Zlength ll) shs)) as Hshi by (apply Forall_Znth; auto; lia).
+    rewrite sublist_next in H10, H11 by lia.
+    inv H10; inv H11.
+    destruct (sepalg_list.list_join_assoc1 (sepalg.join_comm H17) H19) as (sh' & ? & Hsh').
+    destruct (sepalg_list.list_join_assoc1 (sepalg.join_comm H15) H18) as (gsh' & ? & Hgsh').
+    assert (Znth (Zlength ll) gshs <> Share.bot).
     { intro X; contradiction bot_unreadable.
       rewrite <- X; apply Forall_Znth; auto; lia. }
-    destruct (sepalg_list.list_join_assoc1 (sepalg.join_comm H14) H16) as (sh' & ? & Hsh').
-    destruct (sepalg_list.list_join_assoc1 (sepalg.join_comm H13) H17) as (gsh' & ? & Hgsh').
-    forward_spawn _thread_func (thread_lock i) (sh1, Znth i shs, Znth i gshs, g, thread_lock i, gv).
-    { erewrite <- lock_inv_share_join; try apply Hsh; auto.
-      unshelve erewrite <- (lock_inv_share_join _ _ _ _ _ _ _ Hsh'); auto.
-      { eapply readable_share_list_join; eauto. }
-      unshelve erewrite <- (ghost_part_share_join _ _ _ _ O O _ _ Hgsh'); auto.
-      { intro; subst.
-        contradiction bot_unreadable.
-        eapply readable_share_list_join; eauto. }
+    assert (gsh' <> Share.bot).
+    { intro X; contradiction bot_unreadable.
+      rewrite <- X; eapply readable_share_list_join; eauto. }
+    sep_apply lock_inv_isptr; Intros.
+    forward_spawn _thread_func (ptr_of ht) (Znth (Zlength ll) shs, gsh2, ht, Znth (Zlength ll) gshs, h, g, gv).
+    { erewrite <- lock_inv_share_join; try apply gsh1_gsh2_join; auto.
+      erewrite <- field_at_share_join; try apply Hsh'.
+      change O with (O + O)%nat.
+      erewrite <- ctr_handle_share_join; try apply Hgsh'; auto; simpl.
       entailer!. }
-    { subst thread_lock; simpl.
-      apply isptr_is_pointer_or_null; rewrite isptr_offset_val; auto. }
-    Exists sh' gsh'; entailer!.
+    { simpl; auto. }
+    Exists sh' gsh' (ll ++ [ht]); entailer!.
+    { split; [autorewrite with sublist; auto | rewrite map_app, Forall_app; repeat constructor; auto]. }
     apply sepcon_derives.
     - rewrite Z2Nat.inj_add, upto_app by lia.
       rewrite iter_sepcon_app; simpl.
-      rewrite Z2Nat.id, Z.add_0_r by lia; cancel.
-    - rewrite <- Z.sub_add_distr.
-      subst thread_lock.
-      rewrite field_address0_offset, offset_offset_val.
-      rewrite Z.mul_succ_r with (m := i); cancel.
-      { rewrite field_compatible0_cons.
-        split; [lia|].
-        destruct H7 as (? & ? & ? & ? & ?).
-        repeat split; auto.
-        + hnf.
-          destruct (gv _thread_lock); try contradiction; simpl in *.
-          rewrite Z.max_r by lia.
-          rewrite Ptrofs.add_unsigned, Ptrofs.unsigned_repr;
-            rewrite Ptrofs.unsigned_repr; unfold N in *; try rep_lia.
-        + destruct (gv _thread_lock); try contradiction; simpl in *.
-          inv H23; try discriminate.
-          constructor.
-          intros; rewrite Ptrofs.add_unsigned, Ptrofs.unsigned_repr;
-            rewrite Ptrofs.unsigned_repr; unfold N in *; try rep_lia.
-          simpl; rewrite <- Z.add_assoc, Zred_factor4.
-          apply H29; lia. }
-    - apply Z2Nat.inj; try lia.
-      rewrite Nat2Z.id, Z2Nat.inj_sub by lia; simpl; lia. }
-  rewrite !sublist_nil, Zminus_diag; Intros shx gshx.
-  inv H8; inv H9.
+      rewrite Z2Nat.id, Z.add_0_r, app_Znth2, Zminus_diag, Znth_0_cons by (tauto || lia); cancel.
+      rewrite Zlength_correct, Nat2Z.id; apply iter_sepcon_derives; intros ??%In_upto.
+      rewrite <- Zlength_correct in *; autorewrite with sublist; auto.
+    - rewrite upd_complete_gen' by tauto; autorewrite with sublist; apply derives_refl. }
+  rewrite !sublist_nil, Zminus_diag; Intros shx gshx ll.
+  inv H9; inv H10.
   forward_for_simple_bound N (EX i : Z, EX sh : share, EX gsh : share,
     PROP (sepalg_list.list_join shx (sublist 0 i shs) sh;
-          sepalg_list.list_join gshx (sublist 0 i gshs) gsh) LOCAL (gvars gv)
-    SEP (lock_inv sh (gv _ctr_lock) (cptr_lock_inv g (gv _ctr));
-         ghost_part g gsh (Z.to_nat i);
-         iter_sepcon (fun j => lock_inv sh2 (thread_lock j)
-           (thread_lock_inv sh1 (Znth j shs) (Znth j gshs) g (gv _ctr) (gv _ctr_lock) (thread_lock j)))
+          sepalg_list.list_join gshx (sublist 0 i gshs) gsh)
+    LOCAL (lvar _thread_lock (tarray (tptr t_lock) N) v_thread_lock; gvars gv)
+    SEP (library.mem_mgr gv; field_at sh t_counter (DOT _lock) (ptr_of h) (gv _c);
+         spacer Ews 4 8 (gv _c); ctr_handle gsh h g (gv _c) (Z.to_nat i);
+         iter_sepcon (fun j => lock_inv gsh1 (Znth j ll)
+           (thread_lock_inv (Znth j shs) gsh2 (Znth j gshs) g (gv _c) h (Znth j ll)))
            (sublist i N (upto (Z.to_nat N)));
-         data_at_ Ews (tarray tlock i) (gv _thread_lock))).
-  { unfold N; computable. }
-  { rewrite !sublist_nil; Exists shx gshx; entailer!.
+         data_at Tsh (tarray (tptr t_lock) N) (map ptr_of ll) v_thread_lock; has_ext tt))%assert.
+  { rewrite !sublist_nil, sublist_same, app_nil_r by (auto; lia).
+    Exists shx gshx; entailer!.
     { split; constructor. }
-    rewrite !data_at__eq, !data_at_zero_array_eq; auto. simpl; cancel. }
+    apply derives_refl. }
   { (* second loop *)
     forward.
-    replace (force_val _) with (thread_lock i)
-      by (simpl; rewrite sem_add_pi_ptr_special; auto; unfold N in *; simpl in *; rep_lia).
-    Opaque upto.
-    rewrite sublist_next with (i0 := i) by (auto; rewrite Zlength_upto, Z2Nat.id; lia); simpl.
-    rewrite Znth_upto by (simpl; unfold N in *; lia).
-    forward_call (thread_lock i, sh2, thread_lock_inv sh1 (Znth i shs) (Znth i gshs) g
-      (gv _ctr) (gv _ctr_lock) (thread_lock i)).
+    { entailer!. apply isptr_is_pointer_or_null, Forall_Znth; auto.
+      rewrite Zlength_map; simpl in *; replace (Zlength ll) with N; auto. }
+    Opaque N.
+    rewrite sublist_next; auto; simpl.
+    rewrite Znth_upto by auto.
+    forward_call (gsh1, Znth i ll, thread_lock_inv (Znth i shs) gsh2 (Znth i gshs) g (gv _c) h (Znth i ll)).
+    { rewrite Znth_map by (simpl in *; lia); entailer!. }
     { cancel. }
-    unfold thread_lock_inv at 2; unfold thread_lock_R.
-    rewrite selflock_eq; Intros.
-    forward_call (thread_lock i, Ews, sh1, thread_lock_R (Znth i shs) (Znth i gshs) g (gv _ctr) (gv _ctr_lock),
-      thread_lock_inv sh1 (Znth i shs) (Znth i gshs) g (gv _ctr) (gv _ctr_lock) (thread_lock i)).
+    unfold thread_lock_inv at 2; unfold thread_lock_R, selflock; Intros.
+    forward.
+    forward_call freelock_self (gsh1, gsh2, Znth i ll, thread_lock_R (Znth i shs) (Znth i gshs) g (gv _c) h).
+    { rewrite Znth_map by (simpl in *; lia); entailer!. }
     { lock_props.
-      unfold thread_lock_inv, thread_lock_R.
-      erewrite <- (lock_inv_share_join _ _ Ews); try apply Hsh; auto; cancel. }
+      unfold thread_lock_inv, thread_lock_R, selflock; cancel. }
     erewrite <- sublist_same with (al := shs) in Hshs by eauto.
     erewrite <- sublist_same with (al := gshs) in Hgshs by eauto.
     rewrite sublist_split with (mid := i) in Hshs, Hgshs by lia.
-    rewrite sublist_next with (i0 := i) in Hshs by lia.
-    rewrite sublist_next with (i0 := i) in Hgshs by lia.
+    rewrite sublist_next with (i := i) in Hshs by lia.
+    rewrite sublist_next with (i := i) in Hgshs by lia.
     rewrite app_cons_assoc in Hshs, Hgshs.
     apply sepalg_list.list_join_unapp in Hshs as (sh' & Hshs1 & ?).
     apply sepalg_list.list_join_unapp in Hgshs as (gsh' & Hgshs1 & ?).
@@ -367,38 +346,27 @@ Proof.
     apply list_join_eq with (c := sh) in J; auto; subst.
     apply list_join_eq with (c := gsh) in Jg; auto; subst.
     rewrite <- sepalg_list.list_join_1 in J1, Jg1.
-    gather_SEP 3 1; erewrite lock_inv_share_join; eauto.
-    gather_SEP 3 2; erewrite ghost_part_share_join; eauto.
     rewrite !(sublist_split 0 i (i + 1)), !sublist_len_1 by lia.
     Exists sh' gsh'; entailer!.
     { split; eapply sepalg_list.list_join_app; eauto; econstructor; eauto; constructor. }
-    rewrite Z2Nat.inj_add by lia.
-    rewrite !sepcon_assoc; apply sepcon_derives; [apply derives_refl|].
-    rewrite sepcon_comm, sepcon_assoc; apply sepcon_derives; [apply derives_refl|].
-    rewrite !data_at__tarray.
-    rewrite Z2Nat.inj_add, <- list_repeat_app by lia.
-    erewrite split2_data_at_Tarray_app by (rewrite Zlength_list_repeat; auto; lia).
-    rewrite Z.add_simpl_l; cancel.
-    simpl; erewrite data_at_singleton_array_eq by eauto.
-    rewrite field_address0_offset.
-    cancel.
-    { rewrite field_compatible0_cons; split; auto; try lia.
-      apply field_compatible_array_smaller0 with (n' := N); auto; lia. }
-    { intro X; contradiction unreadable_bot.
-      rewrite <- X; eapply readable_share_list_join; eauto. }
-    { intro X; contradiction unreadable_bot.
-      rewrite <- X; apply Forall_Znth; auto; lia. }
-    { eapply readable_share_list_join; eauto. }
-    { apply Forall_Znth; auto; lia. } }
+    unfold thread_lock_R.
+    sep_eapply field_at_share_join; [apply sepalg.join_comm; eauto|].
+    sep_eapply ctr_handle_share_join; try (apply sepalg.join_comm; eauto).
+    { intros X; contradiction unreadable_bot; rewrite <- X; apply Forall_Znth; auto; lia. }
+    { intros X; contradiction unreadable_bot; rewrite <- X.
+      eapply readable_share_list_join; eauto. }
+    rewrite Z2Nat.inj_add, plus_comm by lia; simpl; unfold thread_lock_inv, thread_lock_R, selflock; cancel.
+    { rewrite Zlength_upto; lia. } }
   Intros sh' gsh'.
   eapply list_join_eq in Hshs; [|erewrite <- (sublist_same 0 N shs) by auto; eauto].
   eapply list_join_eq in Hgshs; [|erewrite <- (sublist_same 0 N gshs) by auto; eauto].
   subst.
-  forward_call (g, Z.to_nat N, gv).
+  forward_call (h, g, Z.to_nat N, gv).
   forward.
-  rewrite Z2Nat.id; [|unfold N; computable].
+  rewrite Z2Nat.id by auto.
   (* We've proved that t is N! *)
   forward.
+  { repeat sep_apply data_at_data_at_; cancel. }
 Qed.
 
 Definition extlink := ext_link_prog prog.
@@ -409,11 +377,16 @@ Lemma prog_correct:
   semax_prog prog tt Vprog Gprog.
 Proof.
 prove_semax_prog.
-do 7 semax_func_cons_ext.
+semax_func_cons_ext.
+{ simpl.
+  Intros h.
+  unfold PROPx, LOCALx, SEPx, local, lift1; simpl; unfold liftx; simpl; unfold lift; Intros.
+  destruct ret; unfold eval_id in H0; simpl in H0; subst; simpl; [|contradiction].
+  saturate_local; apply prop_right; auto. }
+do 4 semax_func_cons_ext.
 semax_func_cons body_init_ctr.
 semax_func_cons body_dest_ctr.
 semax_func_cons body_incr.
 semax_func_cons body_thread_func.
 semax_func_cons body_main.
 Qed.
-
